theory/Hoare.v
@@ -1,0 +1,223 @@
+(** * Hoare: Hoare Logic, Part I *)
+
+Set Warnings "-notation-overridden,-parsing".
+Require Import Coq.Bool.Bool.
+Require Import Coq.Arith.Arith.
+Require Import Coq.Arith.EqNat.
+Require Import Coq.omega.Omega.
+From PLF Require Import Imp.
+From PLF Require Import Maps.
+Definition Assertion := state -> Prop.
+
+Definition assert_implies (P Q : Assertion) : Prop :=
+  forall st, P st -> Q st.
+
+Notation "P ->> Q" := (assert_implies P Q)
+                        (at level 80) : hoare_spec_scope.
+Open Scope hoare_spec_scope.
+
+Notation "P <<->> Q" :=
+  (P ->> Q /\ Q ->> P) (at level 80) : hoare_spec_scope.
+
+Notation "a -[ b ]=>  c" := (b / a \\ c) (at level 80) : hoare_spec_scope.
+
+(* The definition of the under triple *)
+
+Definition under_hoare_triple
+           (P:Assertion) (c:com) (Q:Assertion) : Prop :=
+  forall st', Q st' -> exists st, P st /\ st -[c]=> st'.
+
+Notation "|= [[ P ]]  c  [[ Q ]]" :=
+  (under_hoare_triple P c Q) (at level 90, c at next level)
+    : hoare_spec_scope.
+
+Reserved Notation " |- [[ P ]]  c  [[ Q ]]"
+         (at level 40, c at next level).
+
+Definition assn_sub X a P : Assertion :=
+  fun (st : state) =>
+    P (st & { X  --> aeval st a }).
+
+Notation "P [ X |-> a ]" := (assn_sub X a P) (at level 10).
+
+Definition assn_sub_rev X a P: Assertion :=
+  fun (st : state) => exists v, st X = aeval (st & {X --> v}) a /\ P (st & {X --> v}).
+
+Notation "P [ X /== a ]" := (assn_sub_rev X a P) (at level 10).
+
+Definition bassn b : Assertion :=
+  fun st => (beval st b = true).
+
+Lemma bexp_eval_true : forall b st,
+    beval st b = true -> (bassn b) st.
+Proof.
+  intros b st Hbe.
+  unfold bassn. assumption.  Qed.
+
+Lemma bexp_eval_false : forall b st,
+    beval st b = false -> ~ ((bassn b) st).
+Proof.
+  intros b st Hbe contra.
+  unfold bassn in contra.
+  rewrite -> contra in Hbe. inversion Hbe.  Qed.
+
+Lemma bexp_eval_false_rev : forall b st,
+     ~ bassn b st -> beval st b = false.
+Proof.
+  intros b st.
+  destruct (beval st b) eqn:H; intros; auto.
+  - exfalso. auto.
+Qed.
+
+Lemma bexp_eval_true_rev : forall b st,
+     bassn b st -> beval st b = true.
+Proof.
+  intros b st H.
+  inversion H. auto.
+Qed.
+
+Hint Resolve bexp_eval_true : core.
+Hint Resolve bexp_eval_false : core.
+Hint Resolve bexp_eval_false_rev : core.
+Hint Resolve bexp_eval_true_rev : core.
+
+Inductive under_hoare_proof : Assertion -> com -> Assertion -> Prop :=
+| UH_Skip : forall P,
+    |- [[ P ]] SKIP [[P]]
+| UH_Asgn : forall P V a,
+    |- [[ P ]] (V ::= a) [[ P [V /== a] ]]
+| UH_Seq  : forall P c Q d R,
+    |- [[P]] c [[Q]] ->
+    |- [[Q]] d [[R]] ->
+    |- [[P]] (c;; d) [[R]]
+| UH_If_t : forall P Q b c1 c2,
+    |- [[fun st => P st /\ bassn b st]] c1 [[Q]] ->
+    |- [[P]] (IFB b THEN c1 ELSE c2 FI) [[Q]]
+| UH_If_f : forall P Q b c1 c2,
+    |- [[fun st => P st /\ ~(bassn b st)]] c2 [[Q]] ->
+    |- [[P]] (IFB b THEN c1 ELSE c2 FI) [[Q]]
+| UH_Consequence  : forall (P Q P' Q' : Assertion) c,
+    |- [[P']] c [[Q']] ->
+      P' ->> P ->
+      Q ->> Q' ->
+    |- [[P]] c [[Q]]
+| UH_While : forall {A : Type} (R : A -> A -> Prop) M P inv b c,
+    (* well founded order relation R a b: a < b *)
+    well_founded R ->
+    (* Assume M is a ranking function (relation) M st a := ranking function maps st to a.
+       Every state in the invaraint has a rank *)
+    inv ->> (fun st' => exists a', M st' a') ->
+    (* The invaraint should cover the state that is in the precondition and makes the guard to be false *)
+    (fun st => P st /\ ~ (bassn b st)) ->> inv ->
+    (* Any state in the invaraint and not directly reached from the precondition, there exists a pre state
+       1) is in the invaraint
+       2) make the guard to be true
+       3) is well founded. *)
+    (forall a',
+        |- [[fun st => exists a, R a a' /\ M st a /\ inv st /\ bassn b st]] c [[ fun st' => inv st' /\ M st' a' /\ ~ P st']]) ->
+    (* The conjunction of the negation of guard and the invariant is the postcondition *)
+    |- [[P]] WHILE b DO c END [[fun st => inv st /\ ~ (bassn b st)]]
+
+where " |- [[ P ]]  c  [[ Q ]]" := (under_hoare_proof P c Q) : hoare_spec_scope.
+
+Definition uh_while_st := forall {A : Type} (R : A -> A -> Prop) M P b c (Q: Assertion),
+    well_founded R ->
+    (forall st, Q st -> exists a, M a st) ->
+    (forall st' a', Q st' /\ M a' st' ->
+               (exists st a,
+                   (M a st /\ R a a') /\
+                     st -[c]=> st' /\ Q st /\ bassn b st) \/ (~ bassn b st' /\ P st')).
+
+Hint Constructors under_hoare_proof : core.
+Hint Constructors ceval : core.
+Hint Unfold under_hoare_triple : core.
+Hint Unfold assn_sub : core.
+
+Inductive while_prefix (c: com) b : state -> state -> Prop:=
+| While_prefix_nil : forall st, while_prefix c b st st
+| While_prefix_cons : forall st st' st'',
+    bassn b st ->
+    st -[c]=> st' ->
+    while_prefix c b st' st'' -> while_prefix c b st st''.
+
+Hint Constructors while_prefix : core.
+
+Lemma while_prefix_end (c: com) b: forall st st'',
+    while_prefix c b st st'' -> ~ (bassn b st'') -> st -[WHILE b DO c END]=> st''.
+Proof.
+  intros.
+  induction H; eauto.
+Qed.
+
+Lemma while_prefix_rev : forall (c: com) b (st st' st'': state),
+  while_prefix c b st st' ->
+  bassn b st' ->
+  st' -[c]=> st'' ->
+  while_prefix c b st st''.
+Proof.
+  intros.
+  induction H; eauto.
+Qed.
+
+Lemma assertion_destruct: forall (P: Assertion) st, (P st \/ ~ P st).
+Proof. Admitted.
+
+Lemma under_hoare_while: forall {A : Type} (R : A -> A -> Prop) M P Q b c,
+    well_founded R ->
+    Q ->> (fun st' => exists a', M st' a') ->
+    (fun st => P st /\ ~ (bassn b st)) ->> Q ->
+    (forall a',
+        |= [[fun st => exists a, R a a' /\ M st a /\ Q st /\ bassn b st]] c [[ fun st' => Q st' /\ M st' a' /\ ~ P st']]) ->
+    (forall st', Q st' -> exists st, while_prefix c b st st' /\ P st).
+Proof.
+  intros A R M P Q b c Hwellfound HQE H1 Hbody st' HQ'.
+  destruct (HQE st' HQ') as (a' & Hm').
+  generalize dependent st'.
+  induction Hwellfound with a'.
+  intros st' HQ' HM'.
+  destruct (assertion_destruct P st') as [Hbase | Hind].
+  exists st'; split; eauto.
+  destruct (Hbody x st') as (stmid & (a & HR & HM & HQ & HT) & Heval). split; auto.
+  destruct (H0 a HR stmid) as (st & HW & HP); auto.
+  exists st; split; auto.
+  apply while_prefix_rev with stmid; auto.
+Qed.
+
+(* Soundness *)
+Theorem under_hoare_proof_sound  : forall P c Q,
+    |- [[P]] c [[Q]] -> |= [[P]] c [[Q]].
+Proof.
+  intros.
+  induction H; intros st' HQ.
+  - (* skip *)
+    exists st'; split; eauto.
+  - (* assign *)
+    inversion HQ; subst. destruct H as [Hassn HP].
+    exists (st' & {V --> x}); split; eauto.
+    assert (st' = st' & {V --> x; V --> aeval (st' & {V --> x}) a}).
+    rewrite t_update_shadow. rewrite <- Hassn. rewrite t_update_same. auto.
+    rewrite H at 2. auto.
+  - (* seq *)
+    apply IHunder_hoare_proof2 in HQ.
+    destruct HQ as (st_mid & Hmid & Hevalmid).
+    apply IHunder_hoare_proof1 in Hmid.
+    destruct Hmid as (st & HP & HevalP).
+    exists st; split; eauto.
+  - (* if true *)
+    apply IHunder_hoare_proof in HQ.
+    destruct HQ as (st & (HP & HT) & Heval).
+    exists st; split; eauto.
+  - (* if false *)
+    apply IHunder_hoare_proof in HQ.
+    destruct HQ as (st & (HP & HF) & Heval).
+    exists st; split; eauto.
+  - apply H1 in HQ. apply IHunder_hoare_proof in HQ.
+    destruct HQ as (st & HP & Heval).
+    exists st; split; eauto.
+  - (* while *)
+    destruct HQ as [HQ' HF'].
+    assert (exists st, while_prefix c b st st' /\ P st). eapply under_hoare_while; eauto.
+    destruct H4 as (st & HW & HP).
+    exists st. split; auto.
+    apply while_prefix_end; auto.
+Qed.
